dafny/exam2023/Exercise-2.dfy
@@ -1,0 +1,85 @@
+
+//Exercise 2: 5 pts
+// You are given the following definitions
+
+datatype List<T> = Nil | Cons(head:T, tail:List<T>)
+
+predicate sorted(l:List<int>)
+{
+    match l 
+       case Nil         => true
+       case Cons(x, xs) => 
+            match xs 
+               case Nil         => true
+               case Cons(y, ys) => x <= y && sorted(xs)
+}
+
+predicate sortedDec(l:List<int>)
+{
+    match l 
+       case Nil         => true
+       case Cons(x, xs) => 
+            match xs 
+               case Nil         => true
+               case Cons(y, ys) => x >= y && sortedDec(xs)
+}
+
+function elems<T> (l:List<T>) : multiset<T>
+{
+   match l
+      case Nil         => multiset{}
+      case Cons(x, xs) => multiset{x} + elems(xs)
+}
+
+// You must implement and verify function a reverse function satisfying 
+// the specification below. The implementation should use an auxiliary function
+// with an accumulator parameter, so that the time cost should be in O(n)
+
+lemma sortedHeadTailOrderLemma (l:List<int>)
+requires l != Nil
+requires sorted(l)
+ensures forall e | e in elems(l.tail) :: e >= l.head
+{}
+
+function reverse (l:List<int>) : (res:List<int>)
+requires sorted(l)
+ensures  sortedDec(res)
+ensures  elems(res) == elems(l)
+{
+   match l
+      case Nil          => Nil
+      case Cons(x,xs)   =>
+         sortedHeadTailOrderLemma(l);
+         assert elems(reverseAccum(xs, Cons(x,Nil))) == elems(xs) + elems(Cons(x,Nil));
+         reverseAccum(xs, Cons(x,Nil))
+}
+
+lemma sortedDecPrependLemma (x:int, l:List<int>)
+requires sortedDec(l)
+requires forall e | e in elems(l) :: x >= e
+ensures sortedDec(Cons(x,l))
+{
+   if l == Nil {
+      assert sortedDec(Cons(x,l));
+   } else {
+      assert l.head in elems(l);
+      assert x >= l.head;
+   }
+}
+
+function reverseAccum(l:List<int>, lAcc:List<int>) : (res:List<int>)
+requires sorted(l)
+requires sortedDec(lAcc)
+requires forall e1, e2 | e1 in elems(l) && e2 in elems(lAcc) :: e1 >= e2;
+ensures sortedDec(res)
+ensures elems(res) == elems(l) + elems(lAcc)
+{
+   match l
+      case Nil          => lAcc
+      case Cons(x,xs)   =>
+         sortedHeadTailOrderLemma(l);
+         assert x in elems(l);
+         assert forall e | e in elems(lAcc) :: x >= e;
+         sortedDecPrependLemma(x,lAcc);
+         reverseAccum(xs,Cons(x,lAcc))
+}
