dafny/exam2023_check/Exercise-1.dfy
@@ -1,0 +1,93 @@
+
+
+//Exercise 1: 5 pts
+//Given an array of positive integers we want to know if it "evenOdd", 
+// i.e. if it is formed by a (possibly empty) sequence of even numbers 
+//followed by a (possibly empty) sequence of odd numbers
+//In that case we want to return the integer p in [0..v.Length] such that 
+//all elements in v[0..p) are even and those in v[p..v.Length) are odd
+
+//For example: 
+//array v = [2, 1, 7, 5] is evenOdd, and we return p=1
+//array v = [6, 2, 20]  is evenOdd, and we return p=3 
+//array v = [2, 3, 8] is not evenOdd
+//array v = [5, 6] is not evenOdd
+
+
+predicate positive(s:seq<int>)
+{
+    forall k :: 0 <= k < |s| ==> s[k] >= 0
+}
+
+//1. [0.5pt] Define the following predicates 
+
+//All the elements in v[i..j) are even
+predicate even(v:array<int>,i:int,j:int)
+reads v
+requires 0 <= i <= j <= v.Length
+{
+    forall k | i <= k < j :: v[k] % 2 == 0
+}
+
+//All the elements in v[i..j) are odd
+predicate odd(v:array<int>,i:int,j:int)
+reads v
+requires 0 <= i <= j <= v.Length
+{
+    forall k | i <= k < j :: v[k] % 2 == 1
+}
+
+//2. [1.5pt] Write the postcondition of method evenOdd, which returns 
+// - boolean isEvenOdd, which is true if and only if array v is evenOdd as explained above
+// - if isEvenOdd is true, then p is an integer in [0..v.Length] such that 
+//   all elements in v[0..p) are even and those in v[p..v.Length) are odd
+method evenOdd(v:array<int>) returns (isEvenOdd:bool,p:int)
+requires positive(v[0..v.Length])
+ensures isEvenOdd == (exists i | 0 <= i <= v.Length :: even(v,0,i) && odd(v,i,v.Length))
+ensures isEvenOdd ==> (0 <= p <= v.Length)
+ensures isEvenOdd ==> even(v,0,p)
+ensures isEvenOdd ==> odd(v,p,v.Length)
+{
+    isEvenOdd := true;
+    p := 0;
+
+    if (v.Length == 0) {
+        assert even(v,0,0);
+        return;
+    }
+    
+    while (p < v.Length && v[p] % 2 == 0)
+        decreases v.Length - p
+        invariant 0 <= p <= v.Length
+        invariant forall k | 0 <= k < p :: v[k] % 2 == 0
+        invariant even(v,0,p)
+        invariant p == v.Length ==> even(v,0,v.Length)
+        invariant isEvenOdd == even(v,0,p)
+    {
+        if (v[p] % 2 == 0) {
+            p := p + 1;
+        }
+    }
+
+    if (p == v.Length) {
+        return;
+    }
+
+    assert v.Length > 0;
+
+    var q:int := p;
+
+    while (q < v.Length && isEvenOdd)
+        decreases v.Length - q
+        invariant p <= q <= v.Length
+        invariant isEvenOdd == odd(v,p,q)
+    {
+        if (v[q] % 2 == 0) {
+            isEvenOdd := false;
+        }
+        q := q + 1;
+    }
+
+}
+
+//3. [3 pt] Implement and verify method evenOdd
