dafny/session-2/ExerciseFactorial.dfy
@@ -7,24 +7,108 @@ function factorial(n:int):int
 if n == 0 then 1 else n*factorial(n-1)
 }
 
-lemma {:induction n} factorial_Lemma(n:int)  // TODO 
-    decreases n
-	requires n >= 7
-	ensures exp(3,n) < factorial(n)
+lemma factorialLowerBound(n:int)
+requires n > 1
+ensures factorial(n) > 0
 {
-	if n == 7  // base case
-	{
-		assert exp(3, 7) < factorial(7);
-	}
-	else  // inductive case
-	{
-		fact_Lemma(n-1);
+	if n == 2 {
 		
-		assert exp(3, n-1) < factorial(n-1);
+	}
+}
+
+lemma expLowerBound(x:int, n:int)
+requires x > 0
+requires n >= 0
+ensures exp(x,n) > 0
+{}
+
+lemma factorial_LemmaAux1 (n1:int, n2:int, n3:int, n4:int)
+requires n1 > 0 && n2 > 0
+requires n1 <= n3
+requires n2 <= n4
+ensures n1 * n2 <= n3 * n4
+{}
+
+lemma factorial_LemmaAux2 (n1:int, n2:int, n3:int, n4:int, n5:int, n6:int)
+requires n1 > 0 && n2 > 0
+requires n1 < n3
+requires n2 < n4
+requires n5 == n1 * n2
+requires n6 == n3 * n4
+ensures n1 * n2 <= n3 * n4
+ensures n5 <= n6
+{}
+
+lemma {:induction n} factorial_Lemma(n:int)
+decreases n
+requires n >= 7
+ensures exp(3,n) < factorial(n)
+{
+	if (n == 7) {
+		assert exp(3,n) < factorial(n);
+	} else {
+		factorial_Lemma(n-1);
+		assert n > 7;
+		calc == {
+			exp(3,n-1) < factorial(n-1);
+			{ assert 3 < n; }
+			{ assert exp(3,n-1) < factorial(n-1); }
+			{ expLowerBound(3, n-1); }
+			{ factorial_LemmaAux1(3, exp(3,n-1), n, factorial(n-1)); }
+			{ assert 3 * exp(3,n-1) < n * factorial(n-1); }
+			{ assert 3 * exp(3,n-1) == exp(3,n); }
+			exp(3,n) < n * factorial(n-1); 
+		}
+	}
+}
+
+lemma expLessThan_Lemma1(x:int, n:int)
+requires x > 0
+requires n >= 1
+ensures exp(x,n) <= exp(x,n+1)
+{}
+
+lemma expLessThan_Lemma2(x1:int, x2:int, n:int)
+decreases n
+requires x1 > 0 && x2 > 0
+requires x1 <= x2
+requires n >= 1
+ensures exp(x1,n) <= exp(x2,n)
+{
+	if (n == 1) {
+		assert x1 <= x2;
+	} else {
+		expLessThan_Lemma2(x1,x2,n-1);
+		calc == {
+			exp(x1,n-1) <= exp(x2,n-1);
+			// { assert x1 <= x2; }
+			{ expLowerBound(x1,n-1); }
+			{ factorial_LemmaAux1(x1, exp(x1,n-1), x2, exp(x2,n-1)); }
+			x1 * exp(x1,n-1) <= x2 * exp(x2,n-1);
+			// { assert exp(x1,n) == x1 * exp(x1,n-1); }
+			// { assert exp(x2,n) == x2 * exp(x2,n-1); }
+			exp(x1,n) <= exp(x2,n);
+		}
 	}
 }
 
 lemma fact_Lemma(n:int)
-    decreases n
-	requires n >= 1
-	ensures factorial(n) <= exp(n,n)
+decreases n
+requires n >= 1
+ensures factorial(n) <= exp(n,n)
+{
+	if (n == 1) {
+		assert factorial(n) <= exp(n,n);
+	} else {
+		assert n > 1;
+		fact_Lemma(n-1);
+		calc == {
+			factorial(n-1) <= exp(n-1,n-1);
+			// { assert n * factorial(n-1) == factorial(n); }
+			// { assert n - 1 <= n; }
+			{ expLessThan_Lemma2(n-1,n,n-1); }
+			// { assert exp(n-1,n-1) <= exp(n,n-1); }
+			factorial(n-1) <= exp(n,n-1);
+		}
+	}
+}
