dafny/session-3/ExerciseMaximum.dfy
@@ -62,3 +62,55 @@ ensures forall k::0 <= k < v.Length ==> m >= v[k]
     var i := mmaximum(v);
     m := v[i];
 }
+
+///////////////////////////////////////////////
+
+method mfirstMaximum2(v:array<int>) returns (i:int)
+requires v.Length > 0
+ensures 0 <= i < v.Length 
+ensures forall k | 0 <= k < v.Length :: v[i] >= v[k]
+ensures forall l | 0 <= l < i :: v[i] > v[l]
+{
+    var k:int := 0;
+    i := k;
+    // var max:int := v[k];
+
+    while(k < v.Length)
+        decreases v.Length - k
+        invariant 0 <= k <= v.Length
+        invariant 0 <= i < v.Length
+        invariant forall l | 0 <= l < i :: v[i] > v[l]
+        invariant forall j | 0 <= j < k :: v[i] >= v[j]
+    {
+        if (v[k] > v[i])
+        {
+            i := k;
+        }
+        k := k + 1;
+    }
+}
+
+method mlastMaximum2(v:array<int>) returns (i:int)
+requires v.Length > 0
+ensures 0 <= i < v.Length 
+ensures forall k | 0 <= k < v.Length :: v[i] >= v[k]
+ensures forall l | i < l < v.Length :: v[i] > v[l]
+{
+    var k:int := v.Length - 1;
+
+    i := k;
+
+    while (k >= 0)
+        decreases k
+        invariant -1 <= k < v.Length
+        invariant 0 <= i < v.Length
+        invariant forall j | k < j < v.Length :: v[i] >= v[j]
+        invariant forall l | i < l < v.Length :: v[i] > v[l]
+    {
+        if (v[k] > v[i])
+        {
+            i := k;
+        }
+        k := k - 1;
+    }
+}
