dafny/session-6/ExercisePeekSum.dfy
@@ -18,30 +18,29 @@
   else
     peekSum(v,i-1)
  }
-
  
- method mPeekSum(v:array<int>) returns (sum:int)
- requires v.Length > 0
- ensures sum == peekSum(v,v.Length)
- //Implement and verify an O(v.Length) algorithm to solve this problem
- {
-    var i:int:=1;
-    var j:int:=0;  // j is the index of the last peek
-    sum := v[i-1];  // isPeek(v,0) is always true
-    while (i < v.Length)
-      decreases v.Length - i
-      invariant 1 <= i <= v.Length
-      invariant 0 <= j < v.Length
-      invariant j < i  // at each iteration j is always less than i (i.e. j is always a peek)
-      invariant forall k | 0 <= k < i :: v[j] >= v[k]
-      invariant isPeek(v,j)
-      invariant sum == peekSum(v,i)
-    {
-        if (v[i] >= v[j]) {
-            sum := sum + v[i];
-            j := i;
-        }
-        // else sum := sum;
-        i:=i+1;
-    }
- }
+method mPeekSum(v:array<int>) returns (sum:int)
+requires v.Length > 0
+ensures sum == peekSum(v,v.Length)
+//Implement and verify an O(v.Length) algorithm to solve this problem
+{
+  var i:int:=1;
+  var j:int:=0;  // j is the index of the last peek
+  sum := v[i-1];  // isPeek(v,0) is always true
+  while (i < v.Length)
+    decreases v.Length - i
+    invariant 1 <= i <= v.Length
+    invariant 0 <= j < v.Length
+    invariant j < i  // at each iteration j is always less than i (i.e. j is always a peek)
+    invariant forall k | 0 <= k < i :: v[j] >= v[k]
+    invariant isPeek(v,j)
+    invariant sum == peekSum(v,i)
+  {
+      if (v[i] >= v[j]) {
+          sum := sum + v[i];
+          j := i;
+      }
+      // else sum := sum;
+      i:=i+1;
+  }
+}
